so close...

partialImpliesFull.v
@@ -6,14 +6,13 @@ Theorem validateNewerStamp : forall b tid rv rv' wv e0 L H chkpnt HI HV,
 Proof.
   intros b tid rv rv' wv e0 L H chkpnt HI HV H0 H1.
   remember (commit chkpnt HI HV). genDeps{{chkpnt; HI; HV; rv'}}.
-  induction H0; intros; try solve[inv Heqv]. (*not sure why dependent induction doesn't work here...*)
+  induction H0; intros; invertEq. (*not sure why dependent induction doesn't work here...*)
   {constructor. }
-  {inv Heqv. eapply validChkpnt; eauto. inv H1; constructor; eauto.
-   omega. }
-  {inv Heqv. eapply validRead; eauto. inv H1; econstructor; eauto. omega. }
-  {inv Heqv. eapply validWrite; eauto. }
+  {eapply validChkpnt; eauto. inv H1; constructor; auto. omega. }
+  {eapply validRead; eauto. inv H1; econstructor; eauto. omega. }
+  {eapply validWrite; eauto. omega. }
 Qed. 
-
+ 
 (*simulate a replay relation under full abort semantics as long as the endpoint
 **log is valid*)
 Theorem replayFMulti : forall b b' H C C' e0 L e L' e' H' chkpnt tid HI HV, 
@@ -26,12 +25,16 @@ Proof.
   genDeps{{chkpnt; HI; HV; C'}}. dependent induction H0; intros.
   {constructor. }
   {dependent destruction H1.
-   {dependent destruction H5. econstructor. eauto. unfold f_step.
+   {invertHyp. econstructor. eauto. unfold f_step.
     eapply c_transStep. econstructor; eauto. }
-   {dependent destruction H5. econstructor. eauto. unfold f_step.
+   {invertHyp. econstructor. eauto. unfold f_step.
     eapply c_transStep. econstructor; eauto. }
-   {dependent destruction H5. transEq. invertEq. exfalso.
-    eapply validInvalidStamp; eauto. }
+   {dependent destruction H6; invertHyp.
+    {econstructor; eauto. transEq. invertEq. exfalso.
+     eapply validInvalidStamp; eauto. }
+    {econstructor; eauto. transEq. invertEq. exfalso.
+     eapply validInvalidStamp; eauto. }
+   }
    {eapply validateAcquiredLock in H5; eauto. invertHyp. econstructor.
     eauto. eapply c_transStep. eapply t_writeLocked; eauto. }
    {econstructor. eauto. eapply c_transStep. eapply t_atomicIdemStep; eauto. }
@@ -39,60 +42,118 @@ Proof.
   }
 Qed. 
 
-Ltac invertEq :=
-  match goal with
-    | H1:?a = ?b, H2:?a = ?c |- _ => rewrite H1 in H2; inv H2
-  end. 
-
 Theorem falseLogHeapsSame : forall tid rv wv e0 L H chkpnt HI HV,
     @validate tid rv wv e0 false L H (commit chkpnt HI HV) ->
     H = HI /\ H = HV.
 Proof.
   intros. dependent induction H0; auto. 
 Qed. 
+
+Theorem validateValidatePropAbort :
+  forall b l tid rv wv e0 HI v' lock H HV L chkpnt,
+    validStamp tid rv lock -> Log.notIn l b L ->
+    validate tid rv wv e0 L H (commit chkpnt HI HV) ->
+    validate tid rv wv e0 L (update H l v' lock) (commit chkpnt (update HI l v' lock) (update HV l v' lock)). 
+Proof.
+  intros. remember (commit chkpnt HI HV).
+  genDeps{{chkpnt; HI; HV; v'; lock; l}}.
+  induction H2; intros; inv Heqv.
+  {constructor. }
+  {invertHyp. destruct (Nat.eq_dec l l0).
+   {subst. destruct chkpnt. econstructor. heapUnfold. simplEq l0 l0. eauto. 
+    inv H4. constructor. constructor; auto. eauto. }
+   {destruct chkpnt. econstructor. heapUnfold. simplEq l0 l. eauto.
+    auto. eauto. }
+  }
+  {invertHyp. destruct (Nat.eq_dec l l0).
+   {subst. econstructor. heapUnfold. simplEq l0 l0. eauto. 
+    inv H4. constructor. constructor; auto. eauto. }
+   {econstructor. heapUnfold. simplEq l0 l. eauto.
+    auto. eauto. }
+  }
+  {invertHyp. rewrite updatecomm.
+   replace (update (update HV l v (Unlocked wv)) l0 v'0 lock) with
+   (update (update HV l0 v'0 lock) l v (Unlocked wv)). 
+   econstructor; eauto. heapUnfold. simplEq l0 l. eauto.
+   apply updatecomm; auto. apply neqSymm. auto. }
+Qed. 
+
+Definition getChkpnt res :=
+  match res with
+  |abort (e', L) H => L
+  |commit (e', L) HI HV => L
+  end. 
+
+Theorem notInChkpnt : forall b tid rv wv e0 L H res l,
+    Log.notIn l b L -> validate tid rv wv e0 L H res ->
+    Log.notIn l false (getChkpnt res). 
+Proof.
+  intros. induction H1; simpl; auto; dependent destruction H0; auto. 
+  {destruct chkpnt. simpl in *. inv H2. }
+  {destruct chkpnt. invertHyp. eauto. }
+  {destruct chkpnt. invertHyp. eauto. }
+  {invertHyp. }
+Qed. 
+
+
+Theorem validateNoWrites : forall tid rv wv e0 L H chkpnt HI HV,
+    @validate tid rv wv e0 false L H (commit chkpnt HI HV) ->
+    H = HI /\ H = HV.
+Proof.
+  intros. dependent induction H0; auto.
+Qed. 
   
 Theorem commitChkpnt : forall tid rv b wv e0 L H e' L' HI HV,
     @validate tid rv wv e0 b L H (commit (e', L') HI HV) ->
-    validate tid rv wv e0 L' HI (commit (e', L') HI HI).
-Proof.
-  intros. remember (e', L'). remember (commit p HI HV).
-  genDeps{{e'; L'; HI; HV; p}}. induction H0; intros.
-  {subst. inv Heqv. constructor. }
-Admitted.
-
+    exists chkpnt, validate tid rv wv e0 L' HI (commit chkpnt HI HI).
+Proof. 
+  intros. remember (commit (e', L') HI HV). 
+  genDeps{{e'; L'; HI; HV}}. induction H0; intros; inv Heqv; eauto. 
+  {repeat econstructor. }
+  {(*valid checkpoint*)
+    copy H2.  apply validateNoWrites in H2. invertHyp. subst. eauto. }
+  {assert(commit (e', L') HI HV = commit (e', L') HI HV). auto.
+   apply IHvalidate in H4. invertHyp. exists x. destruct x. 
+   eapply validateValidatePropAbort. constructor. auto.
+   eapply notInChkpnt in H2; eauto. simpl in H2. auto. auto. }
+Qed. 
 
 Theorem validateValidate : forall tid rv b wv e0 L H e' L' H',
     @validate tid rv wv e0 b L H (abort (e', L') H') ->
-    exists HV, validate tid rv wv e0 L' H' (commit (e', L') H' HV).
+    exists chkpnt, validate tid rv wv e0 L' H' (commit chkpnt H' H').
 Proof.
   intros. remember (abort (e',L') H'). genDeps{{e'; L'; H'}}.
-  induction H0; intros; try solve[inv Heqv]. 
-  {(*invalidChkpnt*) inv Heqv. eapply commitChkpnt in H2; eauto. }
-  {inv Heqv. eapply commitChkpnt in H2. econstructor. eauto. }
+  induction H0; intros.
+  {inv Heqv. }
+  {inv Heqv. }
+  {inv Heqv. eapply commitChkpnt in H2; eauto. }
+  {inv Heqv. }
+  {inv Heqv. eapply commitChkpnt in H2; eauto. }
+  {inv Heqv. }
   {inv Heqv. eauto. }
-  {inv Heqv. assert(abort (e', L') HI = abort (e', L') HI). auto.
-   eapply IHvalidate in H2. invertHyp. Admitted. 
+  {(*propogate abort*)
+    invertEq. assert(abort (e', L') HI = abort (e', L') HI). auto.
+    apply IHvalidate in H4. invertHyp. exists x.  
+    eapply validateValidatePropAbort; eauto.
+    constructor. auto. eapply notInChkpnt in H2; eauto. simpl in *. auto. }
+Qed. 
 
-
-
-   
 (*full abort can simulate partial abort*)
 Theorem partialImpliesFull : forall C H T C' H' T', 
                                p_step C H T C' H' T' -> poolRewind C H T ->
                                f_multistep C H T C' H' T'. 
 Proof.
   intros. induction H0.
-  {inv H0. econstructor. unfold f_step. eapply c_liftedStep.
-   eapply f_abortStep; eauto. dependent destruction H1.
-   copy H3. eapply abortRewind in H2; eauto. 
-   eapply validateRewindHeapEq in H2; eauto. subst. copy H3.
-   eapply validateValidate in H3; eauto.
-   invertHyp. eapply validateNewerStamp with (rv' := C) in H5; eauto.
-   eapply replayFMulti in H5; eauto.
-   rewrite multistep_rev_eq. eauto. omega. }
+  {inv H0. dependent destruction H1. econstructor.
+   eapply c_liftedStep. eapply f_abortStep; eauto. copy H0.
+   eapply validateRewindHeapEq in H0; eauto. simpl in *.
+   subst. copy H4. eapply abortRewind in H4; eauto; try omega.
+   eapply validateValidate in H3. invertHyp.
+   rewrite multistep_rev_eq. eapply validateNewerStamp in H5.
+   eapply replayFMulti; eauto. omega. }
   {econstructor. eapply c_transStep; eauto. constructor. }
-  {inv H1. eapply IHc_step in H4. eapply multi_L. eauto. } 
-  {inv H1. eapply IHc_step in H5. eapply multi_R. eauto. }
+  {inv H1. eapply IHc_step in H5. eapply multi_L. eauto. } 
+  {inv H1. eapply IHc_step in H6. eapply multi_R. eauto. }
   {econstructor. eapply c_forkStep; eauto. constructor. } 
   {econstructor. eapply c_allocStep; eauto. constructor. }
   {econstructor. eapply c_commitStep; eauto. constructor. }
