noninterference.v
@@ -1,42 +1,39 @@
 Require Export validateWrite.
 
-Ltac heapUnfold := unfold lookup; unfold update.
-
 Theorem notInUpdate : forall H l v lock l',
     (update H l v lock) l' = None ->
     H l' = None. 
 Proof.
-  intros. unfold update in H0. destruct (Nat.eq_dec l l').
-  {inv H0. }
+  intros. heapUnfold. destruct (Nat.eq_dec l l').
+  {invertEq. }
   {assumption.  }
 Qed.
-
+ 
 Theorem rewindAllocSingle : forall tid H H' b1 b2 S e0 L l v L' e e',
     H' l = None ->
     rewind H (txThread b1 tid S e0 L e) H' (txThread b2 tid S e0 L' e') ->
     exists H'', rewind H'' (txThread b1 tid S e0 L e) (update H' l v (Unlocked 0)) (txThread b2 tid S e0 L' e').
 Proof.
-  intros tid H H' b1 b2 S e0 L l v L' e e' H0 H1. genDeps{{l; v}}. 
-  induction H1; intros.
+  intros. genDeps{{l; v}}. induction H1; intros.
   {repeat econstructor. }
-  {inv H0.
+  {inv H0.  
    {copy H2. eapply IHrewind in H2. invertHyp. exists x. econstructor; eauto.
     econstructor; eauto. destruct (eq_nat_dec l l0).
-    {subst. unfold lookup in H5. transEq. invertEq. }
-    {unfold lookup. unfold update. simplEq l l0. auto. }
+    {subst. heapUnfold. transEq. invertEq. }
+    {heapUnfold. simplEq l l0. auto. }
    }
-   {copy H2. eapply IHrewind in H0. invertHyp. exists x. econstructor. eauto.
+   {copy H2. eapply IHrewind in H0; auto. invertHyp. exists x. econstructor. eauto.
     econstructor; eauto. heapUnfold. destruct (Nat.eq_dec l l0); auto. 
-    subst. unfold lookup in *. transEq. invertEq. }
+    subst. transEq. invertEq. }
    {copy H2. eapply IHrewind in H2. invertHyp. exists x. econstructor.
     eauto. eapply r_readStepInvalid; eauto. destruct (Nat.eq_dec l l0); eauto. 
-    {unfold lookup in *. subst. transEq. invertEq. }
-    {unfold lookup. unfold update. simplEq l l0. eauto. }
+    {heapUnfold. subst. transEq. invertEq. }
+    {heapUnfold. simplEq l l0. eauto. }
    }
    {copy H2. eapply notInUpdate in H2; eauto. eapply IHrewind in H2. invertHyp.
     exists x. econstructor; eauto. destruct (Nat.eq_dec l l0).
-    {subst. unfold update in H0. destruct (Nat.eq_dec l0 l0). invertEq.
-     exfalso. apply n. auto. }
+    {subst. heapUnfold. destruct (Nat.eq_dec l0 l0). invertEq.
+     exfalso. auto. }
     {rewrite <- updatecomm; auto. econstructor; eauto. heapUnfold. simplEq l l0.
      auto. }
    }
@@ -49,8 +46,8 @@ Theorem rewindAlloc : forall C H T l v,
     H l = None -> 
     poolRewind C H T -> poolRewind C (update H l v (Unlocked 0)) T. 
 Proof.
-  intros C H T l v H0 H1. genDeps{{l; v}}. induction H1; intros.
-  {constructor. }
+  intros. genDeps{{l; v}}. induction H1; intros.
+  {constructor. auto. }
   {eapply rewindAllocSingle in H0; eauto.  invertHyp. econstructor; eauto. }
   {econstructor; eauto. }
 Qed.
@@ -58,16 +55,16 @@ Qed.
 (*if tid doesn't own the lock, than it cannot be released after aborting*)
 Theorem lookupValidAbort : forall res b tid rv wv e0 L H l v lock,
     @validate tid rv wv e0 b L H res -> ~locked tid lock ->
-    lookup H l = Some(v, lock) -> 
-    lookup (invalidHeap res) l = Some(v, lock). 
+    H l = Some(v, lock) -> 
+    (invalidHeap res) l = Some(v, lock). 
 Proof.
   intros. genDeps{{lock; v}}. induction H0; intros; simpl in *; eauto. 
   {heapUnfold. destruct (Nat.eq_dec l0 l).
-   {subst. transEq. invertEq. exfalso. apply H2. constructor. }
+   {subst. transEq. invertEq. exfalso. apply H4. constructor. }
    {eauto. }
   }
   {heapUnfold. destruct (Nat.eq_dec l0 l).
-   {subst. transEq. invertEq. exfalso. apply H2. constructor. }
+   {subst. transEq. invertEq. exfalso. apply H4. constructor. }
    {eauto. }
   }
 Qed. 
@@ -79,19 +76,21 @@ Theorem lookupAbortLocked : forall res b tid rv tid' wv e0 L H l v oldV v',
      (invalidHeap res) l = Some(v', Unlocked oldV)). 
 Proof.
   intros. genDeps{{tid'; l; v; oldV; v'}}. induction H0; intros; simpl; auto. 
-  {copy H2. eapply IHvalidate in H2. heapUnfold. destruct (Nat.eq_dec l l0).
-   {subst. simpl in *. unfold lookup in *. transEq. invertEq. right. auto. }
-   {auto. }
+  {copy H4. eapply IHvalidate in H4. destruct (Nat.eq_dec l l0). 
+   {subst. simpl in *. transEq. invertEq. right. heapUnfold.
+    simplEq l0 l0. auto. }
+   {simpl in *. unfold update. simplEq l l0. auto. }
   }
-  {copy H2. eapply IHvalidate in H2. heapUnfold. destruct (Nat.eq_dec l l0).
-   {subst. simpl in *. unfold lookup in *. transEq. invertEq. right. auto. }
+  {copy H4. eapply IHvalidate in H4. unfold update. destruct (Nat.eq_dec l l0).
+   {subst. simpl in *. transEq. invertEq. right. auto. }
    {eauto. }
   }
 Qed. 
- 
+
 Theorem abortRewindSingleNI : forall b' H H' HI b tid chkpnt rv e0 L e L' e0' rv' wv' tid',
     @validate tid' rv' wv' e0' b' L' H (abort chkpnt HI) ->
     rewind H' (txThread false tid rv e0 NilLog e0) H (txThread b tid rv e0 L e) ->
+    tid' <> tid -> 
     exists H'', rewind H'' (txThread false tid rv e0 NilLog e0) HI (txThread b tid rv e0 L e) .
 Proof.
   intros. genDeps{{tid'; rv'; wv'; e0'; L'; HI}}.
@@ -101,53 +100,77 @@ Proof.
    {(*r_readChkpnt*)
      copy H5. eapply IHrewind in H5. Focus 2. eauto. invertHyp.
      exists x. econstructor. eauto. econstructor; eauto.
-     eapply lookupValidAbort in H6. Focus 3. eauto. 
-     simpl in *. assumption. intro. inv H5. dependent destruction H4.
-     admit. (*we need tid <> tid'*)
-   }
+     eapply lookupValidAbort in H7; eauto. dependent destruction H4.
+     intro. inv H4. exfalso; auto. intro. inv H5. auto. }
    {(*r_readNoChkpnt*)
      copy H5. eapply IHrewind in H5. Focus 2. eauto. invertHyp.
      exists x. econstructor. eauto. econstructor; eauto.
-     eapply lookupValidAbort in H6. Focus 3. eauto. 
-     simpl in *. assumption. intro. inv H5. dependent destruction H4.
-     admit. (*we need tid <> tid'*)
-   }
+     eapply lookupValidAbort in H7; eauto. dependent destruction H4.
+     intro. inv H4. exfalso; auto. intro. inv H5. auto. }
    {(*r_readStepInvalid*)
-     copy H6. eapply IHrewind in H6. Focus 2. eauto. invertHyp. exists x.
-     econstructor. eauto. dependent destruction H5.
-     {eapply lookupValidAbort in H7; eauto. simpl in *.
-      eapply r_readStepInvalid; eauto. constructor. auto. intro. inv H6. }
-     {eapply lookupAbortLocked in H7. Focus 2. eauto. inv H7.
+     copy H7. eapply IHrewind in H7. Focus 2. eauto. Focus 2. auto. invertHyp. exists x.
+     econstructor. eauto. dependent destruction H5. 
+     {eapply lookupValidAbort in H9; eauto. simpl in *.
+      eapply r_readStepInvalid; eauto. constructor. auto. intro. inv H7. }
+     {eapply lookupAbortLocked in H9; eauto. inv H9.
       {simpl in *. eapply r_readStepInvalid; eauto. constructor. auto. }
       {simpl in *. destruct (ge_dec rv s'). 
-       {inv H3. econstructor; eauto. constructor. assumption. }
-       {inv H3. eapply r_readStepInvalid; eauto. constructor. constructor.
-        omega. }
+       {inv H3.
+        {dependent destruction H6; econstructor; eauto. constructor.
+         auto. constructor. auto. }
+        {omega. }
+       }  
+       {inv H3.
+        {eapply r_readStepInvalid; eauto. constructor. constructor.
+         omega. }
+        {eapply r_readStepInvalid; eauto. constructor. constructor. auto. }
+       }
       }
      }
    }
-   {
+   {(*r_writeLocked*)
+     
+ 
+
+
 
      admit. }
    {eapply IHrewind in H3. Focus 2. eauto. invertHyp. exists x. econstructor.
-    eauto. econstructor; eauto. }
+    eauto. eapply r_atomicIdemStep; eauto. auto. }
    {eapply IHrewind in H3. Focus 2. eauto. invertHyp. exists x. econstructor.
-    eauto. eapply r_betaStep; eauto. }
+    eauto. eapply r_betaStep; eauto. auto. }
   }
 Admitted. 
 
-      
+Ltac solveIn :=
+  simpl;
+   match goal with
+   | H:In ?A (Intersection ?A ?S1 ?S2) ?x |- _ => inv H; try solveIn
+   | H:In ?A (Singleton ?A ?x) ?y |- _ => inv H; try solveIn
+   | |- In ?A (Intersection ?A ?S1 ?S2) ?x => constructor; solveIn
+   | |- In ?A (Union ?A ?S1 ?S2) ?x => (apply Union_introl; solveIn) || (apply Union_intror; solveIn)
+   | |- In ?A (Singleton ?A ?x) ?x => constructor
+   | _ => assumption
+   | H : In ?A (Empty_set ?A) ?x |- _ => inv H
+   | H : In ?A (Union ?A ?S1 ?S2) ?x |- _ => inv H; solveIn
+   end.
+
 Theorem abortRewindNI : forall tid b rv wv e0 C L H T chkpnt HI,
     @validate tid rv wv e0 b L H (abort chkpnt HI) ->
+    Disjoint nat (Singleton nat tid) (ids T) ->
     poolRewind C H T -> poolRewind (S C) HI T.
 Proof.
-  intros. genDeps{{tid; rv; wv; e0; L; b; HI}}.
-  induction H1; intros.
-  {constructor. }
-  {eapply abortRewindSingleNI in H2; eauto. invertHyp. econstructor.
-   eassumption. omega. }
-  {constructor; eauto. }
-Qed.
+  intros. genDeps{{tid; rv; wv; e0; L; b; HI}}. induction H2; intros.
+  {constructor. auto. }
+  {assert(tid0 <> tid). intro. subst. inv H4. specialize (H5 tid).
+   apply H5. constructor; constructor.  
+   eapply abortRewindSingleNI in H3; eauto. invertHyp. econstructor.
+   eassumption. omega. auto. }
+  {constructor. auto. eapply IHpoolRewind1; eauto. simpl in *.
+   constructor. intros. intro. inv H2. specialize (H4 x). apply H4.
+   solveIn. eapply IHpoolRewind2; eauto. constructor. intros.
+   intro. solveIn. inv H2. specialize (H3 x). apply H3. solveIn. }
+Qed. 
 
 Theorem commitUnowned : forall b tid rv wv e0 L H chkpnt HI HV l v lock,
     @validate tid rv wv e0 b L H (commit chkpnt HI HV) ->
@@ -157,8 +180,8 @@ Proof.
   intros. remember (commit chkpnt HI HV). genDeps{{HI; HV; chkpnt; l; v; lock}}. 
   induction H0; intros; inv Heqv0; eauto. 
   {heapUnfold. destruct (Nat.eq_dec l l0).
-   {subst. unfold lookup in *. transEq. invertEq. 
-    exfalso. apply H2. constructor. }
+   {subst. transEq. invertEq. 
+    exfalso. apply H4. constructor. }
    {eauto. }
   }
 Qed. 
@@ -172,62 +195,192 @@ Proof.
   intros. remember(commit chkpnt HI HV).
   genDeps{{chkpnt; HI; HV; l; v; oldV; v'; tid'}}. 
   induction H0; intros; inv Heqv0; eauto. 
-  {heapUnfold. destruct (Nat.eq_dec l l0).
-   {subst. unfold lookup in *. transEq. inv H0. auto. }
+  {unfold update. destruct (Nat.eq_dec l l0).
+   {subst. transEq. invertEq. auto. }
    {eauto. }
+  }
+Qed. 
+
+Theorem commitWriteNI :
+  forall b1 b2 tid' rv' wv' e0' L' l v v' tid rv L0 L lock lock' H chkpnt HI HV,
+    @acquireLock l v' tid rv b1 L0 lock lock' L -> tid <> tid' ->
+    H l = Some(v', lock) ->
+    validate tid' rv' wv' e0' L' (update H l v lock') (commit chkpnt HI HV) ->
+    exists HI' HV', @validate tid' rv' wv' e0' b2 L' H (commit chkpnt HI' HV') /\
+    HV = (update HV' l v lock') /\ HV' l = Some(v', lock). 
+Proof.
+  intros. remember (update H l v lock'). remember (commit chkpnt HI HV).
+  genDeps{{b1; tid; rv; v'; lock; L; H; l; v; lock'; chkpnt; HI; HV}}. 
+  induction H3; intros; subst; inv Heqv0. 
+  {repeat econstructor. auto. }
+  {copy H6. eapply IHvalidate in H6; eauto. invertHyp. exists x. exists x0.
+   split; auto. heapUnfold. destruct (Nat.eq_dec l0 l).
+   {invertEq. dependent destruction H; dependent destruction H1. 
+    exfalso; auto. exfalso; auto. }
+   {econstructor; eauto. }
+  }
+  {copy H6. eapply IHvalidate in H6; eauto. invertHyp. exists x. exists x0.
+   split; auto. heapUnfold. destruct (Nat.eq_dec l0 l).
+   {invertEq. dependent destruction H; dependent destruction H1. 
+    exfalso; auto. exfalso; auto. }
+   {econstructor; eauto. }
+  }
+  {copy H5. eapply IHvalidate in H5; eauto. invertHyp. exists (update x l v' (Unlocked oldV)).
+   exists (update x0 l v (Unlocked wv')). heapUnfold.
+   destruct (Nat.eq_dec l0 l).
+   {invertEq. dependent destruction H7; exfalso; auto. }
+   {split. econstructor; eauto. split. rewrite updatecomm; eauto. heapUnfold.
+    simplEq l l0. auto. }
   }
 Qed. 
 
 Theorem commitRewindSingleNI : forall b' H H' HI b tid chkpnt rv e0 L e L' e0' rv' C tid' HV,
     @validate tid' rv' C e0' b' L' H (commit chkpnt HI HV) -> rv < C ->
     rewind H' (txThread false tid rv e0 NilLog e0) H (txThread b tid rv e0 L e) ->
+    tid <> tid' ->
     exists H'', rewind H'' (txThread false tid rv e0 NilLog e0) HV (txThread b tid rv e0 L e) .
 Proof.
   intros. intros. genDeps{{tid'; rv'; C; e0'; L'; HI; HV}}.
   dependent induction H2; intros.
   {repeat econstructor. }
   {dependent destruction H0.
-   {copy H6. eapply commitUnowned in H6; eauto. eapply IHrewind in H7.
+   {copy H6. eapply commitUnowned in H6; eauto. eapply IHrewind in H8.
     Focus 2. eauto. invertHyp. exists x. econstructor; eauto.
-    econstructor; eauto. auto. intro. dependent destruction H4.
-    {inv H8. (*we need tid <> tid'*) admit. }
-    {inv H8. }
-   }
-   {copy H6. eapply commitUnowned in H6; eauto. eapply IHrewind in H7.
+    econstructor; eauto. auto. auto. intro. dependent destruction H4.
+    inv H9. exfalso; auto. inv H9. }
+   {copy H6. eapply commitUnowned in H6; eauto. eapply IHrewind in H8.
     Focus 2. eauto. invertHyp. exists x. econstructor; eauto.
-    econstructor; eauto. auto. intro. dependent destruction H4.
-    {inv H8. (*we need tid <> tid'*) admit. }
-    {inv H8. }
-   }
-   {copy H7. eapply IHrewind in H7. Focus 2. eauto. invertHyp.
+    econstructor; eauto. auto. auto. intro. dependent destruction H4.
+    inv H9. exfalso; auto. inv H9. }
+   {copy H8. eapply IHrewind in H8; auto. invertHyp.
     exists x. econstructor; eauto. dependent destruction H5.
-    {eapply commitUnowned in H8; eauto. 
+    {eapply commitUnowned in H10; eauto. 
      inv H3. eapply r_readStepInvalid; eauto. constructor.
-     constructor. auto. intro. inv H7. }
-    {inv H3. eapply commitMaybeOwned in H8; eauto. inv H8. 
-     {eapply r_readStepInvalid; eauto. constructor. constructor.
-      auto. }
-     {eapply r_readStepInvalid; eauto. constructor. constructor.
-      auto. }
+     constructor. auto. intro. inv H8. }
+    {inv H3.
+     {eapply commitMaybeOwned in H10; eauto. inv H10. 
+      {eapply r_readStepInvalid; eauto. constructor. auto. constructor.
+       auto. }
+      {eapply r_readStepInvalid; eauto. constructor. constructor.
+       auto. }
+     }
+     {eapply commitMaybeOwned in H10; eauto. inv H10.
+      {econstructor; eauto. constructor. auto. constructor. auto. }
+      {econstructor; eauto. constructor. auto. constructor. auto. }
+     }
     }
-    auto. }
-   {admit. }
+   }
+   {eapply commitWriteNI in H6; eauto. invertHyp. eapply IHrewind in H8; eauto.
+    invertHyp. exists x1. econstructor; eauto. econstructor; eauto. }
    {eapply IHrewind in H4. invertHyp. exists x. econstructor. eauto.
-    econstructor; eauto. auto. auto. }
+    eapply r_atomicIdemStep; eauto. auto. auto. auto. }
    {eapply IHrewind in H4. invertHyp. exists x. econstructor. eauto.
-    eapply r_betaStep; eauto. auto. auto. }
+    eapply r_betaStep; eauto. auto. auto. auto. }
   }   
-Admitted.
-
+Qed. 
+          
 Theorem commitRewindNI : forall tid b rv e0 C L H T chkpnt HI HV,
     @validate tid rv C e0 b L H (commit chkpnt HI HV) ->
+    Disjoint nat (Singleton nat tid) (ids T) ->
     poolRewind C H T -> poolRewind (S C) HV T.
-Proof.
-  intros. induction H1.
-  {constructor. }
-  {eapply commitRewindSingleNI in H1; eauto. invertHyp.
-   econstructor; eauto. }
-  {constructor; auto. }
+Proof. 
+  intros. induction H2.
+  {constructor. auto. }
+  {assert(tid <> tid0). intro. subst. inv H1. specialize (H5 tid0).
+   apply H5. solveIn. eapply commitRewindSingleNI in H2; eauto.
+   invertHyp. econstructor; eauto. }
+  {constructor; auto.
+   {apply IHpoolRewind1. constructor. intros. intro. inv H3.
+    inv H1. specialize (H3 x). apply H3. solveIn. }
+   {apply IHpoolRewind2. constructor. intros. intro. inv H3.
+    inv H1. specialize (H3 x). apply H3. solveIn. }
+  }
 Qed. 
-
-   
+  
+Theorem writeSingleNI : forall b' b tid rv e0 L H H' e l v v' tid' rv' L' lock lock' L'',
+    @acquireLock l v' tid' rv' b' L' lock lock' L'' ->
+    rewind H' (txThread false tid rv e0 NilLog e0) H
+           (txThread b tid rv e0 L e) ->
+    H l = Some(v', lock) -> tid' <> tid ->
+    exists H'', rewind H'' (txThread false tid rv e0 NilLog e0) (update H l v lock')
+                  (txThread b tid rv e0 L e).
+Proof. 
+  intros. genDeps{{l; v'; tid'; rv'; L'; lock; lock'; L''; b'; v}}. 
+  dependent induction H1; intros.
+  {repeat econstructor. }
+  {dependent destruction H0.
+   {copy H6. eapply IHrewind with (v := v0) in H6; auto. invertHyp.
+    exists x. destruct (Nat.eq_dec l l0).
+    {subst. transEq. invertEq.
+     dependent destruction H4; dependent destruction H8. 
+     {exfalso; auto. }
+     {econstructor; eauto. eapply r_readStepInvalid; eauto.
+      Focus 2. heapUnfold. simplEq l0 l0. auto. constructor.
+      auto. constructor; auto. constructor. }
+    }
+    {econstructor; eauto. eapply r_readChkpnt; eauto. heapUnfold. simplEq l0 l.
+     eauto. }
+   }
+   {copy H6. eapply IHrewind with (v := v0) in H6; auto. invertHyp.
+    exists x. destruct (Nat.eq_dec l l0).
+    {subst. transEq. invertEq.
+     dependent destruction H4; dependent destruction H8. 
+     {exfalso; auto. }
+     {econstructor; eauto. eapply r_readStepInvalid; eauto.
+      Focus 2. heapUnfold. simplEq l0 l0. auto. constructor.
+      auto. constructor; auto. constructor. }
+    }
+    {econstructor; eauto. eapply r_readNoChkpnt; eauto. heapUnfold. simplEq l0 l.
+     eauto. }
+   }
+   {copy H8. eapply IHrewind with (v := v0) in H8; auto. invertHyp.
+    exists x. destruct (Nat.eq_dec l l0).
+    {subst. transEq. invertEq.
+     dependent destruction H10; dependent destruction H5.
+     {inv H3.
+      {econstructor; eauto. eapply r_readStepInvalid; eauto.
+       Focus 2. heapUnfold. simplEq l0 l0. auto. constructor.
+       auto. constructor; auto. }
+      {econstructor; eauto. eapply r_readStepInvalid; eauto.
+       Focus 2. heapUnfold. simplEq l0 l0. eauto. constructor.
+       auto. constructor. auto. }
+     }
+     {econstructor; eauto. eapply r_readStepInvalid. eauto. Focus 2.
+      heapUnfold. simplEq l0 l0. auto. constructor. auto. constructor.
+      auto. auto. }
+    }
+    {econstructor; eauto. eapply r_readStepInvalid. eauto. Focus 2.
+     heapUnfold. simplEq l0 l. eauto. auto. auto. auto. }
+   }
+   {(*r_writelocked*)
+     heapUnfold. destruct (Nat.eq_dec l l0).
+     {invertEq. dependent destruction H4; dependent destruction H6; exfalso; auto. }
+     {copy H6. eapply IHrewind in H6; eauto. invertHyp. exists x.
+      econstructor; eauto. rewrite updatecomm; auto. econstructor; eauto.
+      heapUnfold. simplEq l0 l. auto. }
+   }
+   {eapply IHrewind in H4; auto. invertHyp. exists x. econstructor; eauto.
+    eapply r_atomicIdemStep; eauto. }
+   {eapply IHrewind in H4; auto. invertHyp. exists x. econstructor; eauto.
+    eapply r_betaStep; eauto. }
+  }
+Qed. 
+  
+Theorem writeNI : forall b lock lock' L' l v v' tid rv  C L H T,
+    Disjoint nat (Singleton nat tid) (ids T) ->
+    @acquireLock l v' tid rv b L lock lock' L' ->
+    H l = Some(v', lock) ->
+    poolRewind C H T -> poolRewind C (update H l v lock') T.
+Proof.
+  intros. induction H3.
+  {repeat constructor. auto. }
+  {assert(tid <> tid0). intro. subst. inv H0. specialize (H6 tid0).
+   apply H6. solveIn. eapply writeSingleNI in H3; eauto. invertHyp.
+   econstructor; eauto. }
+  {constructor. auto.
+   {apply IHpoolRewind1. constructor. intros. intro. inv H4.
+    inv H0. specialize (H4 x). apply H4. solveIn. }
+   {apply IHpoolRewind2. constructor. intros. intro. inv H4.
+    inv H0. specialize (H4 x). apply H4. solveIn. }
+  }
+Qed.
