stepPreservesRewind.v
@@ -1,4 +1,4 @@
-Require Export noninterference. 
+Require Export stepPreservesUniqueness. 
 
 Theorem validInvalidStamp : forall tid S lock,
                               validStamp tid S lock ->
@@ -11,7 +11,7 @@ Qed.
 Theorem rewindNewerStamp : forall S C H1 H2 b1 b2 tid e0 L1 L2 t1 t2 HI HV chkpnt,
                              rewind H1 (txThread b1 tid S e0 L1 t1)
                                     H2 (txThread b2 tid S e0 L2 t2) ->
-                             S < C -> @validate tid S C e0 b2 L2 H2 (commit chkpnt HI HV) ->
+                             C >= S -> @validate tid S C e0 b2 L2 H2 (commit chkpnt HI HV) ->
                              rewind H1 (txThread b1 tid C e0 L1 t1)
                                     H2 (txThread b2 tid C e0 L2 t2). 
 Proof.
@@ -19,17 +19,21 @@ Proof.
   {constructor. }
   {dependent destruction H1.
    {(*r_readChkpnt*)
-     inv H6. econstructor. eapply IHrewind; eauto. 
-     eapply r_readChkpnt; eauto. rewrite H14 in H3. inv H3.
-     inv H17; econstructor. omega. }
+     invertHyp. econstructor. eapply IHrewind; eauto. 
+     eapply r_readChkpnt; eauto. transEq. invertEq. 
+     inv H8; constructor; omega. }
    {(*r_readNoChkpnt*)
-     dependent destruction H6. econstructor; eauto. 
+     invertHyp. econstructor; eauto. 
      eapply r_readNoChkpnt; eauto. transEq. invertEq.
-     inv H7; econstructor; eauto. omega. }
+     inv H8; econstructor; eauto. omega. }
    {(*r_readStepInvalid*)
-     dependent destruction H7. transEq. invertEq. exfalso.
-     eapply validInvalidStamp; eauto. }
-   { (*r_writeLocked*) 
+     dependent destruction H6.
+     {invertHyp. transEq. invertEq.
+      exfalso. eapply validInvalidStamp; eauto. }
+     {invertHyp. transEq. invertEq.
+      exfalso. eapply validInvalidStamp; eauto. }
+   }
+   {(*r_writeLocked*) 
      copy H4. eapply validateAcquiredLock in H4; eauto. invertHyp.
      econstructor. eapply IHrewind; eauto. 
      eapply r_writeLocked; eauto. 
@@ -42,46 +46,57 @@ Proof.
 Qed. 
 
 Theorem poolRewindNewerStamp : forall C C' H T,
-    poolRewind C H T -> C' > C -> poolRewind C' H T. 
+    poolRewind C H T -> C' >= C -> poolRewind C' H T. 
 Proof.
   intros. induction H0.
-  {constructor. }
-  {econstructor; eauto. omega. }
+  {constructor. omega. }
+  {econstructor; eauto. omega. omega. }
   {econstructor; eauto. }
 Qed. 
-    
+
 Theorem f_rewindNoninterference : forall C H C' H' T T' T2,
     f_step C H T C' H' T' -> poolRewind C H T2 ->
-    poolRewind C' H' T2.
+    Disjoint nat (ids T) (ids T2) -> poolRewind C' H' T2.
 Proof.
-  intros C H C' H' T T' T2 H0 H1. generalize dependent T2.
-  induction H0; intros; eauto. 
+  intros. generalize dependent T2.
+  induction H0; intros.
   {(*if someone else aborts, then we can still rewind*)
     inv H0. eapply abortRewindNI; eauto. }
-  {inv H0; auto.  
-   {admit. }
-  }
+  {inv H0; auto. simpl in *. eapply writeNI; eauto. }
+  {simpl in *. eapply IHc_step. auto. constructor.
+   intros. intro. inv H2. specialize (H4 x). apply H4.
+   solveIn. }
+  {simpl in *. eapply IHc_step. auto. constructor.
+   intros. intro. inv H2. specialize (H4 x). apply H4.
+   solveIn. }
+  {eapply poolRewindNewerStamp; eauto. }
   {eapply rewindAlloc; auto. }
   {eapply commitRewindNI; eauto. }
   {eapply poolRewindNewerStamp; eauto. }
+  {auto. }
   {eapply poolRewindNewerStamp; eauto. }
-Admitted. 
+Qed. 
 
 Theorem p_rewindNoninterference : forall C H C' H' T T' T2,
     p_step C H T C' H' T' -> poolRewind C H T2 ->
-    poolRewind C' H' T2.
-Proof.
-  intros C H C' H' T T' T2 H0 H1. generalize dependent T2.
+    Disjoint nat (ids T) (ids T2) -> poolRewind C' H' T2.
+Proof.  
+  intros. generalize dependent T2.
   induction H0; intros; eauto. 
-  {inv H0. eapply abortRewindNI; eauto. }
-  {inv H0; auto.  
-   {admit. }
-  }
+  {inv H0. simpl in *. eapply abortRewindNI; eauto. }
+  {inv H0; auto. eapply writeNI; eauto. }
+  {simpl in *. eapply IHc_step. auto. constructor.
+   intros. intro. inv H2. specialize (H4 x). apply H4.
+   solveIn. }
+  {simpl in *. eapply IHc_step. auto. constructor.
+   intros. intro. inv H2. specialize (H4 x). apply H4.
+   solveIn. }
+  {eapply poolRewindNewerStamp; eauto. }
   {eapply rewindAlloc; auto. }
   {eapply commitRewindNI; eauto. }
   {eapply poolRewindNewerStamp; eauto. }
   {eapply poolRewindNewerStamp; eauto. }
-Admitted.     
+Qed.
 
 (*f_step preserves rewind*)
 Theorem f_stepRewind : forall C H T C' H' T', 
@@ -89,29 +104,29 @@ Theorem f_stepRewind : forall C H T C' H' T',
                        poolRewind C' H' T'. 
 Proof.  
   intros. induction H0; try solve[econstructor;econstructor; econstructor]. 
-  {inv H0. econstructor; econstructor. }
-  {inv H1. inv H0. dependent destruction H0.
-   {(*t_readStep*)
-     eapply rewindSingleInTX; eauto. econstructor. eauto.
-     eapply r_readChkpnt; eauto. }
-   {(*t_readStep*)
-     eapply rewindSingleInTX; eauto. econstructor. eauto.
-     eapply r_readNoChkpnt; eauto. }
-   {(*t_writeLocked*)
-     eapply rewindSingleInTX; eauto. econstructor. eauto.
-     eapply r_writeLocked; eauto. }
-   {(*t_atomicIdemStep*)
-     eapply rewindSingleInTX; eauto. econstructor. eauto.
-     econstructor. auto. }
-   {(*t_betaStep*)
-     eapply rewindSingleInTX; eauto. econstructor. eauto.
-     eapply r_betaStep. auto. }
+  {inv H0. dependent destruction H1. econstructor. constructor.
+   auto. auto. }
+  {dependent destruction H0;
+   match goal with
+   |Hyp : poolRewind ?C ?H (Single ?T) |- _ => dependent destruction Hyp
+   end; econstructor; eauto; econstructor; eauto; try solve[econstructor; eauto]. 
   }
-  {inv H1. constructor. auto. eapply f_rewindNoninterference; eauto. }
-  {inv H1. constructor; auto. eapply f_rewindNoninterference; eauto. }
+  {inv H1. copy H0. eapply f_stepDisjoint in H0; eauto.
+   econstructor; eauto. eapply f_rewindNoninterference; eauto. }
+  {inv H1. copy H0. rewrite DisjointComm in H4. copy H4. eapply f_stepDisjoint in H4; eauto.
+   econstructor; eauto. rewrite DisjointComm. auto.
+   eapply f_rewindNoninterference; eauto. }
   {(*timestamp extension*)
-    dependent destruction H1. eapply rewindSingleInTX; eauto.
-    eapply rewindNewerStamp; eauto. }
+    dependent destruction H1. econstructor. 
+    econstructor. intros. intro. simpl in *. solveIn.
+    omega. econstructor; eauto. econstructor; eauto. }
+  {inv H1. econstructor. auto. }
+  {dependent destruction H1. econstructor; eauto. }
+  {dependent destruction H1. econstructor. econstructor.
+   auto. auto. }
+  {dependent destruction H1. econstructor; eauto. }
+  {dependent destruction H1. econstructor.
+   eapply rewindNewerStamp; eauto. omega. auto. auto. }
 Qed. 
 
 Theorem validateNoWrites : forall tid rv wv e0 L H chkpnt HI HV,
@@ -122,7 +137,7 @@ Proof.
 Qed. 
 
 Theorem commitRewind : forall H  H0 C tid e e' e0 b L L' S HV,
-    @validate tid S C e0 b L H (commit (e', L') H0 HV) -> C > S ->
+    @validate tid S C e0 b L H (commit (e', L') H0 HV) -> C >= S ->
     rewind H0 (txThread false tid S e0 NilLog e0) H (txThread b tid S e0 L e) ->
     rewind H0 (txThread false tid C e0 NilLog e0) H0 (txThread false tid C e0 L' e'). 
 Proof.
@@ -130,13 +145,14 @@ Proof.
   genDeps{{L'; e'; HV; C}}. dependent induction H3; intros. 
   {inv H1. constructor. }
   {dependent destruction H0. 
-   {dependent destruction H6. 
-    copy H8. eapply validateNoWrites in H8; eauto. subst.
+   {invertHyp. copy H9. eapply validateNoWrites in H9; eauto. subst.
     eapply rewindNewerStamp with (C := C); eauto. apply decomposeEq in H1.
     subst. assumption. }
-   {dependent destruction H6. eapply IHrewind; eauto. }
-   {dependent destruction H7. transEq. invertEq. exfalso.
-    eapply validInvalidStamp; eauto. }
+   {invertHyp. eapply IHrewind; eauto. }
+   {dependent destruction H6; invertHyp.
+    {transEq. invertEq. exfalso. eapply validInvalidStamp; eauto. }
+    {transEq. invertEq. exfalso. eapply validInvalidStamp; eauto. }
+   }
    {(*validWrite*)
      eapply validateAcquiredLock in H2; eauto. invertHyp. 
      eapply IHrewind; eauto. }
@@ -153,7 +169,7 @@ Qed.
  * they should be the same.
  **)
 Theorem abortRewind : forall H H0 C tid e e' e0 b L L' S,
-    @validate tid S C e0 b L H (abort (e', L') H0) -> C > S ->
+    @validate tid S C e0 b L H (abort (e', L') H0) -> C >= S ->
     rewind H0 (txThread false tid S e0 NilLog e0) H (txThread b tid S e0 L e) ->
     rewind H0 (txThread false tid C e0 NilLog e0) H0 (txThread false tid C e0 L' e'). 
 Proof. 
@@ -161,26 +177,17 @@ Proof.
   dependent induction H3.
   {dependent destruction H1. inv H0. }
   {dependent destruction H0; eauto.
-   {dependent destruction H5.  (*r_readChkpnt*)
+   {invertHyp. (*r_readChkpnt*)
     (*validChkpnt case is vacuous since it returns a commit *)
-    
     (*invalidChkpnt: this read  is out of date, contradiction...*)
     {transEq. invertEq. exfalso. eapply validInvalidStamp; eauto. } 
     (*readPropAbort: this read is valid, but an earlier one is out of date, use IH*)
-    {dependent destruction H6. eapply IHrewind; eauto. }
-   } 
-   {dependent destruction H5.  (*r_readNoChkpnt*)
-    (*validRead case is vacuous since it returns a commit*)
-
-    (*invalidRead: this read is out of date, contradiction...*)
-    {transEq. invertEq. exfalso. eapply validInvalidStamp; eauto. }
-    (*readPropAbort: this read is valid, but an earlier one is out of date, use IH*)
-    {dependent destruction H6. eapply IHrewind; eauto. }
-   }
-   {dependent destruction H6.   (*r_readStepInvalid*)
-    {(*invalidRead: this read is invalid, but we don't have a checkpoint*)
-      transEq. invertEq. eapply commitRewind; eauto. }
-    {dependent destruction H7. eauto. }
+    eapply IHrewind; eauto. }
+   {invertHyp; eauto. transEq. invertEq. exfalso.
+    eapply validInvalidStamp; eauto. } 
+   {dependent destruction H6; invertHyp; eauto.     (*r_readStepInvalid*)
+    {transEq. invertEq. eapply commitRewind; eauto. }
+    {transEq. invertEq. eapply commitRewind; eauto. }
    }
    {eapply abortAcquiredLock in H5; eauto. }
   }
@@ -191,24 +198,21 @@ Theorem validateRewindHeapEq : forall res b H H'' tid S  L'' e' e0 C,
     rewind H'' (txThread false tid S e0 NilLog e0) H (txThread b tid S e0 L'' e') ->
     invalidHeap res = H''.
 Proof.
-  intros res b H H' tid S L'' e' e0 C H0 H1.
+  intros.
   generalize dependent res. dependent induction H1; intros.
   {dependent destruction H0; auto. inv H1. }
   {dependent destruction H0.
-   {dependent destruction H5.
-    {eapply IHrewind in H7; eauto. }
-    {eapply IHrewind in H7; eauto. }
-    {dependent destruction H6. eapply IHrewind in H5; eauto. }
+   {invertHyp; eauto. 
+    {eapply IHrewind in H8; eauto. }
+    {eapply IHrewind in H8; eauto. }
    }
-   {dependent destruction H5.
-    {eapply IHrewind in H7; eauto. }
-    {eapply IHrewind in H7; eauto. }
-    {dependent destruction H6. eapply IHrewind in H5; eauto. }
-   }
-   {dependent destruction H6.
-    {transEq. invertEq. exfalso. eapply validInvalidStamp; eauto. }
-    {transEq. invertEq. eapply IHrewind in H8; eauto. }
-    {dependent destruction H7. eapply IHrewind in H6; eauto. }
+   {invertHyp; eauto. 
+    {eapply IHrewind in H8; eauto. }
+   } 
+   {dependent destruction H6; invertHyp; eauto; simpl in *. 
+    {eapply IHrewind in H9; eauto. }
+    {eapply IHrewind in H9; eauto. }
+    {eapply IHrewind in H9; eauto. }
    }
    {destruct res.
     {eapply validateAcquiredLock in H4; eauto. invertHyp.
@@ -227,9 +231,10 @@ Theorem p_stepRewind : forall C H T C' H' T',
 Proof. 
   intros. induction H0; try solve[econstructor;econstructor; econstructor]. 
   {(*p_abortStep*)
-    inv H0. dependent destruction H1. econstructor; eauto.
-    eapply abortRewind; eauto. eapply validateRewindHeapEq in H3; eauto.
-    subst. eauto. }
+    inv H0. dependent destruction H1. copy H3.
+    eapply validateRewindHeapEq in H3; eauto. simpl in *.
+    subst. eapply abortRewind in H0; eauto. 
+    econstructor; eauto. omega. }
   {inv H1. inv H0. dependent destruction H0.
    {(*t_readStep*)
      eapply rewindSingleInTX; eauto. econstructor. eauto.
@@ -242,14 +247,25 @@ Proof.
      eapply r_writeLocked. eauto. eauto. assumption. }
    {(*t_atomicIdemStep*)
      eapply rewindSingleInTX; eauto. econstructor. eauto.
-     econstructor. auto. }
+     eapply r_atomicIdemStep; eauto. }
    {(*t_betaStep*)
      eapply rewindSingleInTX; eauto. econstructor. eauto.
      eapply r_betaStep. auto. }
   }
-  {inv H1. constructor. auto. eapply p_rewindNoninterference; eauto. }
-  {inv H1. constructor. eapply p_rewindNoninterference; eauto. auto. }
+  {inv H1. copy H0. eapply p_stepDisjoint in H0; eauto.
+   econstructor; eauto. eapply p_rewindNoninterference; eauto. }
+  {inv H1. copy H0. rewrite DisjointComm in H4. copy H4. eapply p_stepDisjoint in H4; eauto.
+   econstructor; eauto. rewrite DisjointComm. auto.
+   eapply p_rewindNoninterference; eauto. }
   {(*timestamp extension*)
-    dependent destruction H1. eapply rewindSingleInTX; eauto.
-    eapply rewindNewerStamp; eauto. }
+    dependent destruction H1. econstructor. 
+    econstructor. intros. intro. simpl in *. solveIn. omega.
+    econstructor; eauto. econstructor; eauto. }
+  {inv H1. econstructor. auto. }
+  {dependent destruction H1. econstructor; eauto. }
+  {dependent destruction H1. econstructor. econstructor.
+   auto. auto. }
+  {dependent destruction H1. econstructor; eauto. }
+  {dependent destruction H1. econstructor.
+   eapply rewindNewerStamp; eauto. omega. auto. auto. }
 Qed. 
