stepPreservesUniqueness.v
@@ -1,0 +1,138 @@
+Require Export noninterference. 
+Require Import Coq.Sets.Powerset_facts. 
+
+Theorem f_clockMonotonic : forall C H T C' H' T',
+    f_step C H T C' H' T' -> C' >= C.
+Proof.
+  intros. induction H0; auto. inv H0; auto.
+Qed. 
+
+Inductive extension (C C' : nat) (T T' : pool) : Prop :=
+  extension_ : forall extra, ids T' = Union nat (ids T) extra ->
+                        (forall id, In nat extra id -> id >= C) ->
+                        extension C C' T T'. 
+
+
+Theorem unionEmpty : forall A S, Union A S (Empty_set A) = S.
+Proof.
+  intros. apply Extensionality_Ensembles. constructor.
+  intro. intros. solveIn. constructor. auto.
+Qed. 
+
+Theorem f_stepExtension : forall C H T C' H' T',
+    f_step C H T C' H' T' -> extension C C' T T'.
+Proof.
+  intros. induction H0; try solve[(econstructor; simpl; [erewrite unionEmpty; eauto|
+                                                    intros id H999; inv H999])].
+  {inv H0. econstructor. simpl. erewrite unionEmpty. auto.
+   intros. solveIn. }
+  {dependent destruction H0; (econstructor; simpl; [erewrite unionEmpty; eauto|
+                                                    intros id H999; inv H999]). }
+  {inv IHc_step. eapply extension_ with (extra := extra); auto. simpl. 
+   rewrite H1. rewrite Union_associative. rewrite Union_commutative with (A := extra).
+   rewrite <- Union_associative. auto. }
+  {inv IHc_step. eapply extension_ with (extra := extra); auto. simpl. 
+   rewrite H1. rewrite Union_associative. rewrite Union_commutative with (B := extra).
+   rewrite <- Union_associative. auto. }
+  {econstructor. simpl. auto. intros. solveIn. auto. }
+Qed. 
+
+Theorem p_stepExtension : forall C H T C' H' T',
+    p_step C H T C' H' T' -> extension C C' T T'.
+Proof.
+  intros. induction H0; try solve[(econstructor; simpl; [erewrite unionEmpty; eauto|
+                                                    intros id H999; inv H999])].
+  {inv H0. econstructor. simpl. erewrite unionEmpty. auto.
+   intros. solveIn. }
+  {dependent destruction H0; (econstructor; simpl; [erewrite unionEmpty; eauto|
+                                                    intros id H999; inv H999]). }
+  {inv IHc_step. eapply extension_ with (extra := extra); auto. simpl. 
+   rewrite H1. rewrite Union_associative. rewrite Union_commutative with (A := extra).
+   rewrite <- Union_associative. auto. }
+  {inv IHc_step. eapply extension_ with (extra := extra); auto. simpl. 
+   rewrite H1. rewrite Union_associative. rewrite Union_commutative with (B := extra).
+   rewrite <- Union_associative. auto. }
+  {econstructor. simpl. auto. intros. solveIn. auto. }
+Qed. 
+
+Theorem poolRewindLt : forall C H T,
+    poolRewind C H T -> (forall id, In nat (ids T) id -> id < C).
+Proof.
+  induction T; intros; simpl in *; auto. 
+  {inv H0; inv H1;  auto. }
+  {inv H0; inv H1; auto. }
+Qed. 
+
+
+
+Theorem DisjointComm : forall A T1 T2, Disjoint A T1 T2 <-> Disjoint A T2 T1.
+Proof.
+  intros. split; intros. 
+  {constructor. intros. intro. inv H. specialize (H1 x).
+   apply H1. solveIn. }
+  {constructor. intros. intro. inv H. specialize (H1 x).
+   apply H1. solveIn. }
+Qed. 
+    
+Theorem f_stepDisjoint : forall C H T C' H' T' T2,
+    poolRewind C H T -> poolRewind C H T2 ->
+    f_step C H T C' H' T' -> Disjoint nat (ids T) (ids T2) ->
+    Disjoint nat (ids T') (ids T2). 
+Proof.
+  intros. generalize dependent T2. induction H2; intros; simpl in *; eauto. 
+  {inv H1. auto. }
+  {dependent destruction H1; simpl in *; eauto. }
+  {inv H0. apply IHc_step in H8; auto. apply f_stepExtension in H2.
+   inv H2. rewrite H0. constructor. intros. intro. solveIn. inv H5.
+   {inv H2.
+    {inv H3. specialize (H2 x). apply H2. solveIn. }
+    {apply H4 in H5. eapply poolRewindLt in H1; eauto. omega. }
+   }
+   {inv H3. specialize (H5 x). apply H5. solveIn. }
+  }
+  {inv H0. apply IHc_step in H7; auto. apply f_stepExtension in H2.
+   inv H2. rewrite H0. constructor. intros. intro. inv H2. inv H5.
+   {inv H3. specialize (H5 x). apply H5. solveIn. }
+   {inv H2. 
+    {inv H3. specialize (H2 x). apply H2. solveIn. }
+    {apply H4 in H5. eapply poolRewindLt in H1; eauto. omega. }
+   } apply DisjointComm. auto. }
+  {inv H3. inv H0. constructor. intros. intro. inv H0.
+   {inv H3.
+    {inv H0. specialize (H4 x). apply H4. solveIn. }
+    {inv H0. eapply poolRewindLt in H2; eauto. omega. }
+   }
+  }
+Qed. 
+
+Theorem p_stepDisjoint : forall C H T C' H' T' T2,
+    poolRewind C H T -> poolRewind C H T2 ->
+    p_step C H T C' H' T' -> Disjoint nat (ids T) (ids T2) ->
+    Disjoint nat (ids T') (ids T2). 
+Proof.
+  intros. generalize dependent T2. induction H2; intros; simpl in *; eauto. 
+  {inv H1. auto. }
+  {dependent destruction H1; simpl in *; eauto. }
+  {inv H0. apply IHc_step in H8; auto. apply p_stepExtension in H2.
+   inv H2. rewrite H0. constructor. intros. intro. inv H2. inv H5.
+   {inv H2.
+    {inv H3. specialize (H2 x). apply H2. solveIn. }
+    {apply H4 in H5. eapply poolRewindLt in H1; eauto. omega. }
+   }
+   {inv H3. specialize (H5 x). apply H5. solveIn. }
+  }
+  {inv H0. apply IHc_step in H7; auto. apply p_stepExtension in H2.
+   inv H2. rewrite H0. constructor. intros. intro. inv H2. inv H5.
+   {inv H3. specialize (H5 x). apply H5. solveIn. }
+   {inv H2. 
+    {inv H3. specialize (H2 x). apply H2. solveIn. }
+    {apply H4 in H5. eapply poolRewindLt in H1; eauto. omega. }
+   } apply DisjointComm. auto. }
+  {inv H3. inv H0. constructor. intros. intro. inv H0.
+   {inv H3.
+    {inv H0. specialize (H4 x). apply H4. solveIn. }
+    {inv H0. eapply poolRewindLt in H2; eauto. omega. }
+   }
+  }
+Qed. 
+   
