validateWrite.v
@@ -1,5 +1,11 @@
 Require Export semantics.
 
+Ltac heapUnfold :=
+  match goal with
+  |H : update ?h ?l ?v ?lock ?l' = ?x |- _ => unfold update in H; try heapUnfold
+  | |- update ?H ?l ?v ?lock ?l' = ?x => unfold update
+  end.
+
 Theorem validateNotIn : 
   forall tid l v b v'' lock''' rv wv e0 L H lock' chkpnt HI HV,
     Log.notIn l b L -> H l = Some(v'', lock''') -> validStamp tid rv lock''' -> 
@@ -13,23 +19,16 @@ Proof.
   induction H3; intros; try solve[inv Heqv0].
   {inv Heqv0. subst. exists H1. rewrite updateUpdate.
    rewrite updateIdempotent. constructor. eassumption. }
-  {inv Heqv0. dependent destruction H2. eapply IHvalidate in H2; eauto. 
-   invertHyp. unfold lookup in H0. unfold update in H0. 
-   destruct (Nat.eq_dec l0 l). 
-   {subst. econstructor. econstructor; eauto. } 
-   {econstructor. econstructor; eauto. }
-  }
-  {inv Heqv0. dependent destruction H2. eapply IHvalidate in H2; eauto. 
-   invertHyp. unfold lookup in H0. unfold update in H0. 
-   destruct (Nat.eq_dec l0 l). 
-   {subst. econstructor. econstructor; eauto. } 
-   {econstructor. econstructor; eauto. }
-  }
-  {inv Heqv0. dependent destruction H1. 
-   eapply IHvalidate in H1; eauto. invertHyp. econstructor. 
-   rewrite updatecomm; auto. econstructor; eauto. unfold lookup in H0. 
-   unfold update in H0. destruct (Nat.eq_dec l0 l). contradiction. 
-   eassumption. }
+  {inv Heqv0. invertHyp. eapply IHvalidate in H2; eauto.
+   invertHyp. exists x. heapUnfold.
+   destruct(Nat.eq_dec l0 l); subst; econstructor; eauto. }
+  {inv Heqv0. invertHyp. eapply IHvalidate in H2; eauto.
+   invertHyp. exists x. heapUnfold.
+   destruct(Nat.eq_dec l0 l); subst; econstructor; eauto. }
+  {inv Heqv0. invertHyp. eapply IHvalidate in H4; eauto.
+   invertHyp. econstructor. rewrite updatecomm; auto.
+   econstructor; eauto. heapUnfold. destruct (Nat.eq_dec l0 l).
+   contradiction. eassumption. }
 Qed. 
 
 Theorem validateIn :  
@@ -40,25 +39,23 @@ Theorem validateIn :
     exists HV', @validate tid rv wv e0 true L H (commit chkpnt HI HV').
 Proof.
   intros. dependent induction H2.
-  {dependent destruction H0. eapply IHvalidate in H0; eauto. 
-   invertHyp. unfold lookup in H4. unfold update in H4.
-   destruct (Nat.eq_dec l l0).
-   {subst. inv H4. econstructor. econstructor; eauto. }
+  {invertHyp. eapply IHvalidate in H0; eauto. 
+   invertHyp. heapUnfold. destruct (Nat.eq_dec l l0).
+   {subst. invertEq. econstructor. econstructor; eauto. }
    {econstructor. econstructor; eauto. }
   }
-  {dependent destruction H0.
-   {unfold lookup in H3. unfold update in H3.
-    destruct (Nat.eq_dec l0 l0). Focus 2. exfalso; eauto.
-    inv H3. eapply validateNotIn in H0; eauto. invertHyp.
+  {invertHyp. 
+   {heapUnfold. destruct (Nat.eq_dec l0 l0). Focus 2. exfalso; eauto.
+    invertEq. eapply validateNotIn in H0; eauto. invertHyp.
     erewrite <- updateUpdate. econstructor. econstructor; eauto. constructor. }
    {eapply IHvalidate in H1; eauto. invertHyp. econstructor.
-    econstructor; eauto. unfold lookup in H3. unfold update in H3.
-    destruct (Nat.eq_dec l l0). contradiction. eassumption. }
+    econstructor; eauto. heapUnfold. destruct (Nat.eq_dec l l0).
+    contradiction. eassumption. }
   }
 Qed. 
 
 Theorem validateAcquiredLock : forall tid l v v' b rv wv e0 L L' H lock lock' chkpnt HI HV,
-    lookup H l = Some(v', lock) ->
+    H l = Some(v', lock) ->
     acquireLock l v' tid rv L lock lock' L' -> 
     @validate tid rv wv e0 true L' (update H l v lock') (commit chkpnt HI HV) ->
     exists HV', @validate tid rv wv e0 b L H (commit chkpnt HI HV').
@@ -66,9 +63,8 @@ Proof.
   intros tid l v v' b rv wv e0 L L' H lock lock' chkpnt HI HV H0 H1 H2.
   dependent destruction H1. 
   {eapply validateIn in H1; eauto. }
-  {dependent destruction H3. unfold update in H4. unfold lookup in H4. 
-   destruct (Nat.eq_dec l l). inv H4. 
-   eapply validateNotIn in H5; eauto. 
+  {invertHyp. heapUnfold. destruct (Nat.eq_dec l l).
+   invertEq. eapply validateNotIn in H7; eauto. 
    constructor. omega. exfalso; auto. }
 Qed.
 
@@ -82,28 +78,26 @@ Proof.
   intros. remember (update H l v lock'). remember (abort chkpnt HI).
   genDeps{{chkpnt; HI; H; l; v; lock'}}.
   induction H4; intros; try solve[inv Heqv0]. 
-  {inv Heqv0. dependent destruction H5. eapply validateNotIn in H5; eauto. 
-   invertHyp. unfold lookup in H0. unfold update in H0.
-   destruct (Nat.eq_dec l0 l).
-   {subst. inv H0. inv H3. inv H1. exfalso; auto. }
+  {inv Heqv0. invertHyp. eapply validateNotIn in H5; eauto. 
+   invertHyp. heapUnfold. destruct (Nat.eq_dec l0 l).
+   {subst. invertEq. inv H3; inv H1; exfalso; auto. }
    {econstructor; eauto. }
   }
-  {inv Heqv0. dependent destruction H5. eapply validateNotIn in H5; eauto. 
-   invertHyp. unfold lookup in H0. unfold update in H0.
-   destruct (Nat.eq_dec l0 l).
-   {subst. inv H0. inv H3. inv H1. exfalso; auto. }
+  {inv Heqv0. invertHyp. eapply validateNotIn in H5; eauto. 
+   invertHyp. heapUnfold. destruct (Nat.eq_dec l0 l).
+   {subst. invertEq. inv H3; inv H1; exfalso; auto. }
    {econstructor; eauto. }
   }
-  {dependent destruction H0.
-   {dependent destruction H1. eapply IHvalidate in H1; eauto.
-    subst. inv Heqv0. eapply readPropAbort; eauto. constructor. }
-   {inv Heqv0. dependent destruction H1. eapply IHvalidate in H1; eauto.
+  {invertEq. dependent destruction H0.
+   {invertHyp. eapply IHvalidate in H1; eauto.
+    subst. eapply readPropAbort; eauto. constructor. }
+   {invertHyp. eapply IHvalidate in H1; eauto.
     eapply readPropAbort; eauto. constructor. }
-  }
-  {dependent destruction H1. inv Heqv0. eapply IHvalidate in H5; eauto.
-   unfold lookup in H0. unfold update in H0. destruct (Nat.eq_dec l0 l).
-   contradiction. rewrite updatecomm; auto. eapply writePropAbort. auto.
-   eauto. }
+  } 
+  {invertHyp. invertEq. eapply IHvalidate in H9; eauto.
+   heapUnfold. destruct (Nat.eq_dec l0 l). contradiction.
+   rewrite updatecomm; auto. eapply writePropAbort. auto.
+   eauto. auto. auto. }
 Qed.
 
 Theorem abortIn :  
@@ -114,36 +108,34 @@ Theorem abortIn :
     @validate tid rv wv e0 true L H (abort chkpnt HI).
 Proof.
   intros. dependent induction H2.
-  {dependent destruction H0. eapply validateIn in H0; eauto.
-   invertHyp. unfold lookup in H4. unfold update in H4. destruct (Nat.eq_dec l l0).
-   {subst. inv H4. econstructor; eauto. }
+  {invertHyp. eapply validateIn in H0; eauto.
+   invertHyp. heapUnfold. destruct (Nat.eq_dec l l0).
+   {subst. invertEq. econstructor; eauto. }
    {econstructor; eauto. }
   }
-  {dependent destruction H3. dependent destruction H0. eapply IHvalidate in H0; eauto.
+  {dependent destruction H3. invertHyp. eapply IHvalidate in H0; eauto.
    eapply readPropAbort; eauto. constructor. }
-  {dependent destruction H0.
-   {unfold lookup in H3. unfold update in H3. destruct (Nat.eq_dec l0 l0).
-    {inv H3. eapply abortNotIn in H0; eauto. erewrite <- updateUpdate.
+  {invertHyp.
+   {heapUnfold. destruct (Nat.eq_dec l0 l0).
+    {invertEq. eapply abortNotIn in H0; eauto. erewrite <- updateUpdate.
      eapply writePropAbort; eauto. constructor. constructor. }
     {exfalso; auto. }
    }
    {eapply IHvalidate in H1; eauto. eapply writePropAbort; eauto.
-    unfold lookup in H3. unfold update in H3. destruct (Nat.eq_dec l l0).
-    contradiction. eauto. }
+    heapUnfold.  destruct (Nat.eq_dec l l0). contradiction. eauto. }
   }
 Qed. 
 
 Theorem abortAcquiredLock : forall tid l v v' b rv wv e0 L L' H lock lock' chkpnt HI,
-    lookup H l = Some(v', lock) ->
+    H l = Some(v', lock) ->
     acquireLock l v' tid rv L lock lock' L' -> 
     @validate tid rv wv e0 true L' (update H l v lock') (abort chkpnt HI) ->
     @validate tid rv wv e0 b L H (abort chkpnt HI).
 Proof.
   intros. dependent destruction H1. 
   {eapply abortIn in H2; eauto. }
-  {dependent destruction H3. dependent destruction H5.
-   unfold update in H5. unfold lookup in H5. 
-   destruct (Nat.eq_dec l l). inv H5. 
+  {invertHyp. dependent destruction H5.  
+   heapUnfold. destruct (Nat.eq_dec l l). invertEq.
    eapply abortNotIn in H2; eauto. constructor. auto. constructor. 
    exfalso; auto. }
 Qed. 
